Obc.v
@@ -1,6 +1,7 @@
 Require Import Operators.
 Require Export Obc.Syntax.
 Require Export Obc.Semantics.
+Require Export Obc.Typing.
 Require Export Obc.Equiv.
 
 Require Import Rustre.Common.
@@ -9,5 +10,6 @@ Module Type OBC (Ids: IDS) (Op: OPERATORS) (OpAux: OPERATORS_AUX Op).
   Declare Module Export Syn: SYNTAX Ids Op OpAux.
   Declare Module Export Sem: SEMANTICS Ids Op OpAux Syn.
   Declare Module Export Equ: EQUIV Ids Op OpAux Syn Sem.
+  Declare Module Export Typ: TYPING Ids Op OpAux Syn Sem.
 End OBC.
 
